few changes on dsaxioms..

prop10_1_auth.v
@@ -22,100 +22,128 @@ sends <i> < g<sup>b</sup>, sign(skB, g<sup> b </sup>, g<sup>a</sup>) > </i>, and
 </ul>
 #
  *)
+  
+ Notation "( x , y , .. , z )" := (pair .. (pair x y) .. z) .
 
-(** Authentication is modeled as indistinguishability of two protocols, one in which the oracle reveals [TRue] if the given session is completed but no matching session (there exists an attack), and the one in which the oracle always reveals [FAlse]. *)
-
-(** Protocol [Pi1] reveals [FAlse] always. *)
+(** Authentication is modeled as indistinguishability of two protocols, one in which the oracle reveals [TRue] if the given session is completed but no matching session (there exists an attack), and the one in which the oracle always reveals [FAlse]. 
+We use [new] for [TRue] and [acc] for [FAlse] as those are of type message. *)
+(** Protocol [Pi1] reveals [acc] always. *)
 
 (** Frame [phi10] represents initial knowledge of the attacker. *)
 
 Definition phi10 := [msg (G 0); msg (g 0); msg (pk 3); msg (pk 4)].
 Definition mphi10 := (conv_mylist_listm phi10).
 Definition grn (n:nat) := (exp (G 0) (g 0) (r n)).
-Definition x1 := (f mphi10).
-Definition qa00 :=   (ifm ((eqm (to x1) (i 1)) & (eqm (act x1) new)) (grn 1) (ifm (eqm (to x1) (i 2)) (pair (grn 2) (sign (sk 4)  (pair (grn 2) x1))) O)).
+Definition x1 := (f mphi10). 
+Definition qa0 :=   (ifm ((eqm (to x1) (i 1)) & (eqm (act x1) new)) (grn 1) O).
 
 (** Frame [phi11] represents attacker's knowledge during execution of the protocol. *)
 
-Definition phi11 := phi10 ++ [msg qa00].
+Definition phi11 := phi10 ++ [msg qa0].
 Definition mphi11 := (conv_mylist_listm phi11).
-Definition x2 := (f mphi11). 
-Definition qa10 :=  (ifm ((eqm (to x2) (i 1))& (ver (pk 4) (pair (pi1 (x2))  (grn 1))   (pi2 (x2)))) (sign (sk 3) (pair  (grn 1) (pi1 (x2))))  O ).
-Definition qa01:=  (ifm (eqm (to x2) (i 2))& (ver (pk 3) (pair (grn 1) (pi1 x2)) x2) acc O) .
-Definition qa00_s :=  (ifm ((eqm (to x1) (i 1)) & (eqm (act x1) new)) qa10 (ifm (eqm (to x1) (i 2)) qa01 O)).
+Definition x2 := (f mphi11).  
+Definition qa1 :=    (ifm (eqm (to x2) (i 2)) (pair (grn 2) (sign (sk 4)  (pair (grn 2) x1))) O). 
+ Definition qa0_s :=   (ifm ((eqm (to x1) (i 1)) & (eqm (act x1) new)) qa1 O).
 
 (** Frame [phi12] also represents attackers's knowledge during execution of the protocol. *)
+ Definition phi12:= phi11 ++ [msg qa0_s].
 
-Definition phi12:= phi11 ++ [msg qa00_s].
 Definition mphi12 := (conv_mylist_listm phi12).
 Definition x3 := (f mphi12).
-Definition qa20 :=  (ifm (eqm (reveal x3) (i 2))& (notb (eqm (pi1(x2)) (grn 1)) & (eqm x1 (grn 1)))  O O ).
-Definition qa02 := (ifm (eqm (reveal x3) (i 2))& (notb ((eqm (pi1(x2)) (grn 1))) &  (eqm x1 (grn 1)))  O O ).
-Definition qa10_s :=    (ifm ((eqm (to x2) (i 1))& (ver (pk 4) (pair (pi1 (x2))  (grn 1)) (pi2 x2)))  qa20 O ).
-Definition qa01_s := (ifm (eqm (to x2) (i 2))& (ver (pk 3) (pair x1 (grn 1)) x2)& (eqm (pi1(x2)) (grn 1)) & (eqm x1 (grn 1)) qa02 O).
-Definition qa00_ss :=  (ifm ((eqm (to x1) (i 1)) & (eqm (act x1) new)) qa10_s (ifm (eqm (to x1) (i 2)) qa01_s O)).
+  
+Definition qa2 :=  (ifm (eqm (to x3) (i 1))& (ver (pk 4) ( (pi1 x2), (grn 1)) (pi2 x2)) (sign (sk 3) ( (grn 1), (pi1 (x2)))) O).
 
+Definition qa1_s :=   (ifm (eqm (to x2) (i 2)) qa2 O). 
+ Definition qa0_ss :=   (ifm ((eqm (to x1) (i 1)) & (eqm (act x1) new)) qa1_s O).
+(** Frame [phi13] *) 
+ Definition phi13 := phi12 ++ [msg qa0_ss].
+ Definition mphi13 := (conv_mylist_listm phi13).
+ Definition x4 := (f mphi13).
+  
+Definition qa3 :=  (ifm (eqm (to x4) (i 2)) & (ver (pk 3) (x1, (grn 2)) x4) acc O).
+  
+Definition qa2_s :=  (ifm (eqm (to x3) (i 1))& (ver (pk 4) ( (pi1 x2), (grn 1)) (pi2 x2)) qa3 O).
+
+Definition qa1_ss :=   (ifm (eqm (to x2) (i 2)) qa2_s O). 
+Definition qa0_sss :=   (ifm ((eqm (to x1) (i 1)) & (eqm (act x1) new)) qa1_ss O).
+ (** if there is no matching session for a completed responder session, the oracle outputs [new] indicating that there is an attack, other wise outputs [acc] *) 
+  Definition phi14 := phi13 ++ [msg qa0_sss]. 
+ Definition mphi14 := (conv_mylist_listm phi13).
+ Definition x5 := (f mphi14).
+  Definition oracleop1 :=  (ifm (eqm (reveal x5) (i 2))& (notb (eqm x1 (grn 1))&(eqm (pi1(x2)) (grn 2)))  new acc ).
+
+Definition qa3_s :=  (ifm (eqm (to x4) (i 2)) & (ver (pk 3) (x1, (grn 2)) x4) oracleop1 O).
+  
+Definition qa2_ss :=  (ifm (eqm (to x3) (i 1))& (ver (pk 4) ( (pi1 x2), (grn 1)) (pi2 x2)) qa3_s O).
+
+Definition qa1_sss :=   (ifm (eqm (to x2) (i 2)) qa2_ss O). 
+Definition qa0_ssss :=   (ifm ((eqm (to x1) (i 1)) & (eqm (act x1) new)) qa1_sss O).
+ 
 (** Frame [phi13] attacker's knowledge at the end of the protocol. *)
 
-Definition phi13 := phi12 ++ [msg qa00_ss].
 
-(** Protocol Pi2 reveals [TRue] if there is an attack. 
+Definition phi15 := phi14 ++ [msg qa0_ssss].
 
- All the frames in this protocol are equal to the frames in Pi1 except the last one and we define it here. *)
+(** Protocol Pi2 reveals [new] if there is an attack, reveals [acc] otherwise. 
 
-Definition qb20 :=  (ifm (eqm (reveal x3) (i 2))& (notb (eqm (pi1(x2)) (grn 1)) & (eqm x1 (grn 1)))  O O ).
+ All the frames in this protocol are equal to the frames in Pi1 except the last one and we define it here.
+ *)
 
-Definition qb02 := (ifm (eqm (reveal x3) (i 2))& (notb (eqm (pi1(x2)) (grn 1)) & (eqm x1 (grn 1))) new O ).
+(** The oracle always outputs [acc] *)
+  Definition oracleop2 :=  (ifm (eqm (reveal x5) (i 2))& (notb (eqm x1 (grn 1))&(eqm (pi1(x2)) (grn 2)))  acc acc ).
 
-Definition qb10_s :=    (ifm ((eqm (to x2) (i 1))& (ver (pk 4) (pair (pi1 (x2))  (grn 1)) (pi2 x2)))  qb20 O ).
+Definition qb3_s :=  (ifm (eqm (to x4) (i 2)) & (ver (pk 3) (x1, (grn 2)) x4) oracleop2 O).
+  
+Definition qb2_ss :=  (ifm (eqm (to x3) (i 1))& (ver (pk 4) ( (pi1 x2), (grn 1)) (pi2 x2)) qb3_s O).
 
-Definition qb01_s := (ifm (eqm (to x2) (i 2))& (ver (pk 3) (pair x1 (grn 1)) x2)& (eqm (pi1(x2)) (grn 1)) & (eqm x1 (grn 1)) qb02 O).
-
-Definition qb00_ss :=  (ifm ((eqm (to x1) (i 1)) & (eqm (act x1) new)) qb10_s (ifm (eqm (to x1) (i 2)) qb01_s O)).
-Definition phi23 := phi12 ++ [msg qb00_ss].
+Definition qb1_sss :=   (ifm (eqm (to x2) (i 2)) qb2_ss O). 
+Definition qb0_ssss :=   (ifm ((eqm (to x1) (i 1)) & (eqm (act x1) new)) qb1_sss O).
+ 
+Definition phi25 := phi14 ++ [msg qb0_ssss].
 
 (** Proof of [phi13 #### phi23], where [####] is an equivalence relations on mylists. *)
 
-Theorem IND_DH_AUTH:   phi13 #### phi23.
+Theorem IND_DH_AUTH:   phi15 #### phi25.
 
-Proof. unfold phi13, phi23, phi12, phi11, phi10. repeat unfold qa00, qa10 , qa01, qa20, qa02, qa10_s, qa01_s, qa00_s, qa00_ss.
+Proof. repeat unfold phi11, phi12, phi13, phi14, phi15, phi25. repeat  unfold qa0, qa1 , qa2, qa3,  qa0_s, qa1_s, qa2_s, qa3_s. simpl.
+repeat unfold qa0_ss, qa0_sss, qa0_ssss, qb0_ssss, qa1_ss, qa1_sss, qb1_sss, qa2_s, qb2_ss, qa2_ss, qa3_s.
+repeat unfold oracleop1, oracleop2.
+repeat unfold qb3_s, qa1_s, qa3, qa2. 
+assert (qa0_ssss # qb0_ssss).
+repeat unfold qa0_ssss, qa1_sss, qa2_ss, qa3_s, qa3, qb0_ssss, qb1_sss, qb2_ss, qb3_s.
+unfold oracleop1, oracleop2. 
+pose proof( UFCMA 3 (x1 , grn 2) x4).
+simpl in H.
+rewrite H.
+assert( (eqm x1 (grn 1)) ## (eqm  (pi1 (x1 , (grn 2))) (pi1 ((grn 1) , (pi1 x2))))).
+repeat rewrite proj1. reflexivity.
+assert( (eqm (pi1 x2) (grn 2)) ## (eqm (pi2 (grn 1, (pi1 x2))) (pi2 (x1, (grn 2))))).
+repeat rewrite proj2. reflexivity.
+repeat rewrite H0, H1.  
+rewrite <- andB_assoc with (b1:=   (eqm (to x4) (i 2))) (b2:= (eqm (x1, grn 2) (grn 1, pi1 x2))) (b3:=  (ver (pk 3) (grn 1, pi1 x2) x4)). 
+rewrite -> andB_comm with (b2:= (eqm (x1, grn 2) (grn 1, pi1 x2))) (b1:= (eqm (to x4) (i 2))).
+rewrite -> andB_assoc with (b1:= (eqm (x1, grn 2) (grn 1, pi1 x2))). 
+rewrite eqbrmsg_msg' with (m1:= (x1, grn 2)) (m2:= (grn 1, pi1 x2)) (b:=  ((eqm (to x4) (i 2)) & (ver (pk 3) (grn 1, pi1 x2) x4))) (m3:=  (ifm
+                  (eqm (reveal x5) (i 2)) &
+                  (notb
+                     (eqm (pi1 (x1, grn 2)) (pi1 (grn 1, pi1 x2))) &
+                     (eqm (pi2 (grn 1, pi1 x2)) (pi2 (x1, grn 2)))) new acc)) (m4:= O) (m:= (x1, grn 2)).
+rewrite eqbrmsg_msg' with (m1:= (x1, grn 2)) (m2:= (grn 1, pi1 x2)) (b:=  ((eqm (to x4) (i 2)) & (ver (pk 3) (grn 1, pi1 x2) x4))) (m3:=  (ifm
+                    (eqm (reveal x5) (i 2)) &
+                    (notb
+                       (eqm (pi1 (x1, grn 2)) (pi1 (grn 1, pi1 x2))) &
+                       (eqm (pi2 (grn 1, pi1 x2)) (pi2 (x1, grn 2)))) acc acc)) (m4:= O) (m:= (x1, grn 2)).
 simpl.
-repeat unfold qb20, qb02, qb10_s, qb01_s, qb00_ss.
-assert(trm3: (ifm (eqm (to x1) (i 1)) & (eqm (act x1) new)
-         (ifm
-            (eqm (to x2) (i 1)) & (ver (pk 4) (pair (pi1 x2) (grn 1)) (pi2 x2))
-            (ifm
-               (eqm (reveal x3) (i 2)) &
-               (notb (eqm (pi1 x2) (grn 1)) & (eqm x1 (grn 1))) O O) O)
-         (ifm (eqm (to x1) (i 2))
-            (ifm
-               (((eqm (to x2) (i 2)) & (ver (pk 3) (pair x1 (grn 1)) x2)) &
-                (eqm (pi1 x2) (grn 1))) & (eqm x1 (grn 1))
-               (ifm
-                  (eqm (reveal x3) (i 2)) &
-                  (notb (eqm (pi1 x2) (grn 1)) & (eqm x1 (grn 1))) O O) O) O)) # (ifm (eqm (to x1) (i 1)) & (eqm (act x1) new)
-         (ifm
-            (eqm (to x2) (i 1)) & (ver (pk 4) (pair (pi1 x2) (grn 1)) (pi2 x2))
-            (ifm
-               (eqm (reveal x3) (i 2)) &
-               (notb (eqm (pi1 x2) (grn 1)) & (eqm x1 (grn 1))) O O) O)
-         (ifm (eqm (to x1) (i 2))
-            (ifm
-               (((eqm (to x2) (i 2)) & (ver (pk 3) (pair x1 (grn 1)) x2)) &
-                (eqm (pi1 x2) (grn 1))) & (eqm x1 (grn 1))
-               (ifm
-                  (eqm (reveal x3) (i 2)) &
-                  (notb (eqm (pi1 x2) (grn 1)) & (eqm x1 (grn 1))) new O) O) O))).
+assert( (eqm (pi1 (grn 1, pi1 x2)) (pi1 (grn 1, pi1 x2))) ## TRue).
+apply EQmsg with (x:=(pi1 (grn 1, pi1 x2))). reflexivity. repeat rewrite H2. 
+repeat rewrite  IFTRUE_B.
+assert( (eqm (pi2 (grn 1, pi1 x2)) (pi2 (grn 1, pi1 x2))) ## TRue).
+apply EQmsg with (x:= (pi2 (grn 1, pi1 x2))). reflexivity.
+repeat rewrite H3.
+repeat rewrite IFTRUE_B.
+repeat rewrite IFSAME_B.
+repeat rewrite IFFALSE_M. reflexivity. try split; try reflexivity.
+rewrite H. reflexivity. 
+Qed.
 
-assert(vef: (ver (pk 3) (pair x1 (grn 1)) x2) ## FAlse).
-apply (UFCMA 3 (pair x1 (grn 1)) x2);try split; try reflexivity. 
-
-rewrite vef.
-assert(pf:  (((eqm (to x2) (i 2)) & (FAlse)) & (eqm (pi1 x2) (grn 1))) &
-            (eqm x1 (grn 1)) ## FAlse).
-rewrite andB_FAlse_r with (b:= (eqm (to x2) (i 2))).
-rewrite andB_FAlse_l with (b:= (eqm (pi1 x2) (grn 1))).
-rewrite andB_FAlse_l with (b:= (eqm x1 (grn 1))). reflexivity.
-rewrite pf.
-repeat rewrite IFFALSE_M. reflexivity.  rewrite trm3. reflexivity. Qed.
 End dh_auth.
